Dataflow/IsFree/Decide.v
@@ -27,7 +27,7 @@ Fixpoint free_in_lexp (e: lexp) (fvs: PS.t) : PS.t :=
   | Econst c => fvs
   | Evar x => PS.add x fvs
   | Ewhen e x xc => free_in_lexp e (PS.add x fvs)
-  | Eop op eqs => List.fold_left (fun fvs e => free_in_lexp e fvs) eqs fvs
+  | Eop op eqs => Nelist.fold_left (fun fvs e => free_in_lexp e fvs) eqs fvs
   end.
 
 Definition free_in_laexp (lae : laexp) (fvs : PS.t) : PS.t :=
@@ -98,17 +98,18 @@ Proof.
     | right; apply free_in_clock_spec; intuition
     | apply PS.add_spec in H1; destruct H1; subst; intuition
     | right; apply PS.add_spec; intuition ].
-induction les as [| le les]; intro m.
-+ split; intro Hin; auto.
-  destruct Hin as [Hin | Hin]; trivial. inversion_clear Hin. inversion_clear H0.
+induction les as [le | le les]; intro m.
++ simpl. inversion_clear H. rewrite H0. split; intros [Hin | ?]; auto; left.
+  - now do 2 constructor.
+  - inversion_clear Hin. inversion_clear H. assumption.
 + inversion_clear H.
   specialize (IHles H1 (free_in_lexp le m)). rewrite H0 in IHles.
   rewrite IHles. split; intro Hin.
-  - destruct Hin as [Hin | [Hin | Hin]]; tauto || left; constructor;
-    (now left) || now right; inversion_clear Hin.
+  - destruct Hin as [Hin | [Hin | Hin]]; tauto || left; constructor; try now constructor 2. 
+    constructor 3. now inversion_clear Hin.
   - destruct Hin as [Hin | ?]; try tauto; [].
-    inversion_clear Hin.
-    Local Hint Constructors Is_free_in_lexp. inversion_clear H; auto. 
+    Local Hint Constructors Is_free_in_lexp.
+    inversion_clear Hin. inversion_clear H; auto. 
 Qed.
 
 Lemma free_in_lexp_spec':
