Correctness/Proper.v
@@ -77,13 +77,14 @@ Qed.
 Instance translate_lexp_Proper :
   Proper (PS.eq ==> eq ==> eq) translate_lexp.
 Proof.
-  intros M M' HMeq e e' Heq; rewrite <- Heq; clear Heq e'.
-  revert M M' HMeq.
-  induction e using lexp_ind2; intros M M' HMeq; simpl; auto.
-  - rewrite HMeq; auto.
-  - f_equal.
-    induction les; trivial; [].
-    simpl. inversion_clear H. f_equal; auto.
+intros M M' HMeq e e' Heq; rewrite <- Heq; clear Heq e'.
+revert M M' HMeq.
+induction e using lexp_ind2; intros M M' HMeq; simpl; auto.
++ rewrite HMeq; auto.
++ f_equal.
+  induction les; simpl.
+  - f_equal. inversion_clear H. now apply H0.
+  - inversion_clear H. f_equal; auto.
 Qed.
 
 Instance translate_cexp_Proper :
